case_study/RiscvPmp/BlockVer/Spec.v
@@ -33,7 +33,9 @@ From Coq Require Import
 From Equations Require Import
      Equations.
 From Katamaran Require Import
-  (* Iris.Instance *) Iris.BinaryInstance
+     Iris.Instance
+     Iris.BinaryInstance
+     Iris.BinaryWeakestPre
      Iris.Base
      Notations
      Bitvector
@@ -41,12 +43,16 @@ From Katamaran Require Import
      Specification
      MicroSail.ShallowExecutor
      MicroSail.ShallowSoundness
-     MicroSail.SymbolicExecutor
-     MicroSail.RefineExecutor
+     MicroSail.SymbolicExecutor.
+From Katamaran Require Import
+     MicroSail.RefineExecutor.
+From Katamaran Require Import
      MicroSail.Soundness
      RiscvPmp.PmpCheck
      RiscvPmp.IrisModel
+     RiscvPmp.IrisModelBinary
      RiscvPmp.IrisInstance
+     RiscvPmp.IrisInstanceBinary
      RiscvPmp.Machine
      RiscvPmp.Sig
      RiscvPmp.Contracts.
@@ -109,6 +115,7 @@ Module RiscvPmpBlockVerifSpec <: Specification RiscvPmpBase RiscvPmpSignature Ri
   (* Notation asn_pmp_access addr width es m p := (asn.formula (formula_user pmp_access [addr;width;es;m;p])). *)
   (* Notation asn_inv_mmio bytes := (asn.chunk (chunk_user (inv_mmio bytes) [env])). *)
   (* Notation asn_mmio_checked_write bytes a w := (asn.chunk (chunk_user (mmio_checked_write bytes) [a; w])). *)
+  Notation asn_inv_leakage := (asn.chunk (chunk_user inv_leakage [env])).
 
   Definition term_eqb {Σ} (e1 e2 : Term Σ ty_regno) : Term Σ ty.bool :=
     term_binop (bop.relop bop.eq) e1 e2.
@@ -236,28 +243,18 @@ Module RiscvPmpBlockVerifSpec <: Specification RiscvPmpBase RiscvPmpSignature Ri
   Import bv.notations.
 
   Definition sep_contract_rX : SepContractFun rX :=
-    {| sep_contract_logic_variables := ["rs" :: ty_regno; "w" :: ty_word];
+    {| sep_contract_logic_variables := ["rs" :: ty_regno; "reg_val" :: ty_word];
        sep_contract_localstore      := [term_var "rs"];
-      sep_contract_precondition    := asn.formula (formula_secLeak (term_var "rs")) ∗ term_var "rs" ↦ᵣ term_var "w";
+      sep_contract_precondition    := asn.formula (formula_secLeak (term_var "rs")) ∗ term_var "rs" ↦ᵣ term_var "reg_val";
        sep_contract_result          := "result_rX";
-       sep_contract_postcondition   := asn.formula (formula_propeq (term_var "result_rX") (term_var "w")) ∗
-                                       term_var "rs" ↦ᵣ term_var "w";
-    |}.
-
-  Definition sep_contract_rX' : SepContract ["rs'" :: ty.bvec 1] (ty_xlenbits) :=
-    {| sep_contract_logic_variables := ["rs'" :: ty.bvec 1; "w" :: ty_word];
-      sep_contract_localstore      := [term_var "rs'"];
-      sep_contract_precondition    := asn.formula (formula_secLeak (term_var "rs'")) ∗
-                                        asn_reg_ptsto_1 (term_var "rs'") (term_var "w");
-      sep_contract_result          := "result_rX";
-      sep_contract_postcondition   := asn.formula (formula_propeq (term_var "result_rX") (term_var "w")) ∗
-                                        asn_reg_ptsto_1 (term_var "rs'") (term_var "w");
+       sep_contract_postcondition   := asn.formula (formula_propeq (term_var "result_rX") (term_var "reg_val")) ∗
+                                       term_var "rs" ↦ᵣ term_var "reg_val";
     |}.
 
   Definition sep_contract_wX : SepContractFun wX :=
-    {| sep_contract_logic_variables := ["rs" :: ty_regno; "v" :: ty_xlenbits; "w" :: ty_xlenbits];
+    {| sep_contract_logic_variables := ["rs" :: ty_regno; "v" :: ty_xlenbits; "reg_val" :: ty_xlenbits];
        sep_contract_localstore      := [term_var "rs"; term_var "v"];
-       sep_contract_precondition    := term_var "rs" ↦ᵣ term_var "w";
+      sep_contract_precondition    := asn.formula (formula_secLeak (term_var "rs")) ∗ term_var "rs" ↦ᵣ term_var "reg_val";
        sep_contract_result          := "result_wX";
        sep_contract_postcondition   := term_var "result_wX" = term_val ty.unit tt ∗
                                        if: term_eqb (term_var "rs") (term_val ty_regno [bv 0])
@@ -268,55 +265,69 @@ Module RiscvPmpBlockVerifSpec <: Specification RiscvPmpBase RiscvPmpSignature Ri
   Definition sep_contract_fetch_instr : SepContractFun fetch :=
     {| sep_contract_logic_variables := ["a" :: ty_xlenbits; "i" :: ty_ast(* ; "entries" :: ty.list ty_pmpentry *)];
        sep_contract_localstore      := [];
-       sep_contract_precondition    := asn.chunk (chunk_ptsreg pc (term_var "a")) ∗
-                                                 term_var "a" ↦ᵢ term_var "i" ∗
-                                                 (term_val ty.int (Z.of_N minAddr) <= term_unsigned (term_var "a"))%asn ∗
-                                                 (term_binop bop.plus (term_unsigned (term_var "a")) (term_val ty.int (Z.of_nat bytes_per_instr))) <= term_val ty.int (Z.of_N maxAddr) ∗
-                                                 asn_cur_privilege (term_val ty_privilege Machine)(*  ∗ *)
+       sep_contract_precondition    :=
+        asn.formula (formula_secLeak (term_var "a")) ∗ (* Technically this can be concluded from the formula_le, but I think it is better explicit *)
+        asn.chunk (chunk_ptsreg pc (term_var "a")) ∗
+          term_var "a" ↦ᵢ term_var "i" ∗
+          (term_val ty.int (Z.of_N minAddr) <= term_unsigned (term_var "a"))%asn ∗
+          (term_binop bop.plus (term_unsigned (term_var "a")) (term_val ty.int (Z.of_nat bytes_per_instr))) <= term_val ty.int (Z.of_N maxAddr) ∗
+                                                                                                                 asn_cur_privilege (term_val ty_privilege Machine) (* ∗ *)
                                                  (* asn_pmp_entries (term_var "entries") ∗ *)
-                                                 (* asn_pmp_access (term_var "a") (term_val ty_word bv_instrsize) (term_var "entries") (term_val ty_privilege Machine) (term_val ty_access_type Execute) *);
+                                                 (* asn_pmp_access (term_var "a") (term_val ty_word bv_instrsize) (term_var "entries") (term_val ty_privilege Machine) (term_val ty_access_type Execute) *) ∗
+                                                                                                                 asn.chunk (chunk_user inv_leakage [env]);
        sep_contract_result          := "result_fetch";
        sep_contract_postcondition   :=
+        asn.formula (formula_secLeak (term_var "a")) ∗
          asn.chunk (chunk_ptsreg pc (term_var "a")) ∗ term_var "a" ↦ᵢ term_var "i" ∗
-         asn.exist "w" _
-           (term_var "result_fetch" = term_union fetch_result KF_Base (term_var "w") ∗
-                                        asn.chunk (chunk_user encodes_instr [term_var "w"; term_var "i"])) ∗
-           asn_cur_privilege (term_val ty_privilege Machine)(*  ∗ *)
+         asn.exist "encoded_instr" _
+         (term_var "result_fetch" = term_union fetch_result KF_Base (term_var "encoded_instr") ∗
+                                      asn.chunk (chunk_user encodes_instr [term_var "encoded_instr"; term_var "i"])
+         ∗ asn.formula (formula_secLeak (term_var "encoded_instr"))) ∗
+           asn_cur_privilege (term_val ty_privilege Machine) (* ∗ *)
            (* asn_pmp_entries (term_var "entries") *);
     |}.
 
   Definition sep_contract_checked_mem_read {bytes} {H: restrict_bytes bytes} : SepContractFun (@checked_mem_read bytes H) :=
-     {| sep_contract_logic_variables := ["inv" :: ty.bool; "typ" :: ty_access_type; "paddr" :: ty_xlenbits; "w" :: ty_bytes bytes];
+     {| sep_contract_logic_variables := ["inv" :: ty.bool; "typ" :: ty_access_type; "paddr" :: ty_xlenbits; "cmem_val" :: ty_bytes bytes];
       sep_contract_localstore      := [term_var "typ"; term_var "paddr"];
       sep_contract_precondition    :=
+         asn.formula (formula_secLeak (term_var "inv")) ∗
+           asn.formula (formula_secLeak (term_var "paddr")) ∗
         asn.match_bool (term_var "inv")
-          (term_var "paddr" ↦ᵣ[ bytes ] term_var "w")
-          (term_var "paddr" ↦ₘ[ bytes ] term_var "w") ∗
+          (term_var "paddr" ↦ᵣ[ bytes ] term_var "cmem_val")
+          (term_var "paddr" ↦ₘ[ bytes ] term_var "cmem_val") ∗
           (term_val ty.int (Z.of_N minAddr) <= term_unsigned (term_var "paddr"))%asn ∗
-          (term_binop bop.plus (term_unsigned (term_var "paddr")) (term_val ty.int (Z.of_nat bytes))) <= term_val ty.int (Z.of_N maxAddr);
+          (term_binop bop.plus (term_unsigned (term_var "paddr")) (term_val ty.int (Z.of_nat bytes))) <= term_val ty.int (Z.of_N maxAddr) ∗
+                                                                                                           asn.chunk (chunk_user inv_leakage [env]);
       sep_contract_result          := "result_mem_read";
       sep_contract_postcondition   :=
-        term_var "result_mem_read" = term_union (memory_op_result bytes) KMemValue (term_var "w") ∗
-         asn.match_bool (term_var "inv") (term_var "paddr" ↦ᵣ[ bytes ] term_var "w") (term_var "paddr" ↦ₘ[ bytes ] term_var "w");
+         asn.formula (formula_secLeak (term_var "inv")) ∗
+           asn.formula (formula_secLeak (term_var "paddr")) ∗
+           asn.formula (formula_propeq (term_var "result_mem_read") (term_union (memory_op_result bytes) KMemValue (term_var "cmem_val"))) ∗
+         asn.match_bool (term_var "inv") (term_var "paddr" ↦ᵣ[ bytes ] term_var "cmem_val") (term_var "paddr" ↦ₘ[ bytes ] term_var "cmem_val");
     |}.
 
 
   Definition sep_contract_checked_mem_write {bytes} {H: restrict_bytes bytes} : SepContractFun (@checked_mem_write bytes H) :=
-    {| sep_contract_logic_variables := ["inv" :: ty.bool; "paddr" :: ty_xlenbits; "data" :: ty_bytes bytes];
+    {| sep_contract_logic_variables := [(* "inv" :: ty.bool; *) "paddr" :: ty_xlenbits; "data" :: ty_bytes bytes];
       sep_contract_localstore      := [term_var "paddr"; term_var "data"];
       sep_contract_precondition    :=
-        asn.match_bool (term_var "inv")
-          ((* asn_in_mmio bytes (term_var "paddr") ∗ *)
-           term_binop bop.plus (term_unsigned (term_var "paddr")) (term_val ty.int (Z.of_nat bytes)) < (term_val ty.int (Z.of_N (bv.exp2 xlenbits)))(*  ∗ *)
-           (* asn_inv_mmio bytes ∗ *)
-           (* asn_mmio_checked_write bytes (term_var "paddr") (term_var "data") *))
-          (∃ "w", term_var "paddr" ↦ₘ[ bytes ] term_var "w" ∗
+        (* asn.match_bool (term_var "inv") *)
+        (*   ((* asn_in_mmio bytes (term_var "paddr") ∗ *) *)
+        (*     ∃ "w", term_var "paddr" ↦ₘ[ bytes ] term_var "w" ∗ *)
+        (*    term_binop bop.plus (term_unsigned (term_var "paddr")) (term_val ty.int (Z.of_nat bytes)) < (term_val ty.int (Z.of_N (bv.exp2 xlenbits)))(*  ∗ *) *)
+        (*    (* asn_inv_mmio bytes ∗ *) *)
+        (*    (* asn_mmio_checked_write bytes (term_var "paddr") (term_var "data") *)) *)
+        (*   ( *)
+            ∃ "cmem_val", term_var "paddr" ↦ₘ[ bytes ] term_var "cmem_val" ∗
            (term_val ty.int (Z.of_N minAddr) <= term_unsigned (term_var "paddr"))%asn ∗
-           (term_binop bop.plus (term_unsigned (term_var "paddr")) (term_val ty.int (Z.of_nat bytes))) <= term_val ty.int (Z.of_N maxAddr));
+           (term_binop bop.plus (term_unsigned (term_var "paddr")) (term_val ty.int (Z.of_nat bytes))) <= term_val ty.int (Z.of_N maxAddr)(* ) *) ∗
+                                                                                                            asn.chunk (chunk_user inv_leakage [env]) ∗
+    asn.formula (formula_secLeak (term_var "paddr"));
       sep_contract_result          := "result_checked_mem_write";
       sep_contract_postcondition   :=
         term_var "result_checked_mem_write" = term_union (memory_op_result 1) KMemValue (term_val ty_byte [bv 1]) ∗
-        asn.match_bool (term_var "inv") ⊤ (term_var "paddr" ↦ₘ[ bytes ] term_var "data");
+        (* asn.match_bool (term_var "inv") ⊤ *) (term_var "paddr" ↦ₘ[ bytes ] term_var "data");
     |}.
 
   (* Definition sep_contract_pmpCheck {bytes : nat} {H : restrict_bytes bytes} : SepContractFun (@pmpCheck bytes H) := *)
@@ -377,43 +388,51 @@ Module RiscvPmpBlockVerifSpec <: Specification RiscvPmpBase RiscvPmpSignature Ri
   (*   |}. *)
 
   Definition sep_contract_mem_read {bytes} {H : restrict_bytes bytes} : SepContractFun (@mem_read bytes H) :=
-    {| sep_contract_logic_variables := ["inv" :: ty.bool; "typ" :: ty_access_type; "paddr" :: ty_xlenbits; (* "entries" :: ty.list ty_pmpentry; *) "w" :: ty_bytes bytes];
+    {| sep_contract_logic_variables := ["inv" :: ty.bool; "typ" :: ty_access_type; "paddr" :: ty_xlenbits; (* "entries" :: ty.list ty_pmpentry; *) "mem_val" :: ty_bytes bytes];
       sep_contract_localstore      := [term_var "typ"; term_var "paddr"];
       sep_contract_precondition    :=
-        asn.match_bool (term_var "inv") (term_var "paddr" ↦ᵣ[ bytes ] term_var "w") (term_var "paddr" ↦ₘ[ bytes ] term_var "w") ∗
+        asn.formula (formula_secLeak (term_var "inv")) ∗
+          asn.formula (formula_secLeak (term_var "paddr")) ∗
+        asn.match_bool (term_var "inv") (term_var "paddr" ↦ᵣ[ bytes ] term_var "mem_val") (term_var "paddr" ↦ₘ[ bytes ] term_var "mem_val") ∗
           (term_val ty.int (Z.of_N minAddr) <= term_unsigned (term_var "paddr"))%asn ∗
           (term_binop bop.plus (term_unsigned (term_var "paddr")) (term_val ty.int (Z.of_nat bytes))) <= term_val ty.int (Z.of_N maxAddr) ∗
           asn_cur_privilege (term_val ty_privilege Machine)(*  ∗ *)
           (* asn_pmp_entries (term_var "entries") ∗ *)
-          (* asn_pmp_access (term_var "paddr") (term_get_slice_int (term_val ty.int (Z.of_nat bytes))) (term_var "entries") (term_val ty_privilege Machine) (term_var "typ") *);
+          (* asn_pmp_access (term_var "paddr") (term_get_slice_int (term_val ty.int (Z.of_nat bytes))) (term_var "entries") (term_val ty_privilege Machine) (term_var "typ") *) ∗
+          asn.chunk (chunk_user inv_leakage [env]);
       sep_contract_result          := "result_mem_read";
       sep_contract_postcondition   :=
-        term_var "result_mem_read" = term_union (memory_op_result bytes) KMemValue (term_var "w") ∗
-                                       asn.match_bool (term_var "inv") (term_var "paddr" ↦ᵣ[ bytes ] term_var "w") (term_var "paddr" ↦ₘ[ bytes ] term_var "w") ∗
+
+        asn.formula (formula_secLeak (term_var "inv")) ∗
+          asn.formula (formula_secLeak (term_var "paddr")) ∗
+        asn.formula (formula_propeq (term_var "result_mem_read") (term_union (memory_op_result bytes) KMemValue (term_var "mem_val"))) ∗
+                                       asn.match_bool (term_var "inv") (term_var "paddr" ↦ᵣ[ bytes ] term_var "mem_val") (term_var "paddr" ↦ₘ[ bytes ] term_var "mem_val") ∗
           asn_cur_privilege (term_val ty_privilege Machine)(*  ∗ *)
           (* asn_pmp_entries (term_var "entries") *);
     |}.
 
   (* Access type `Write` needed here, as `mem_write_value` calls `pmp_mem_write` with this access type*)
   Definition sep_contract_mem_write_value {bytes} {H: restrict_bytes bytes} : SepContractFun (@mem_write_value bytes H) :=
-    {| sep_contract_logic_variables := ["inv" :: ty.bool; "paddr" :: ty_xlenbits; "data" :: ty_bytes bytes(* ; "entries" :: ty.list ty_pmpentry *)];
+    {| sep_contract_logic_variables := [(* "inv" :: ty.bool; *) "paddr" :: ty_xlenbits; "data" :: ty_bytes bytes(* ; "entries" :: ty.list ty_pmpentry *)];
       sep_contract_localstore      := [term_var "paddr"; term_var "data"];
       sep_contract_precondition    :=
-        asn.match_bool (term_var "inv")
-          ((* asn_in_mmio bytes (term_var "paddr") ∗ *)
-           term_binop bop.plus (term_unsigned (term_var "paddr")) (term_val ty.int (Z.of_nat bytes)) < (term_val ty.int (Z.of_N (bv.exp2 xlenbits))) (* ∗ *)
-           (* asn_inv_mmio bytes ∗ *)
-           (* asn_mmio_checked_write bytes (term_var "paddr") (term_var "data") *))
-          (∃ "w", term_var "paddr" ↦ₘ[ bytes ] term_var "w" ∗
+        (* asn.match_bool (term_var "inv") *)
+        (*   ((* asn_in_mmio bytes (term_var "paddr") ∗ *) *)
+        (*    term_binop bop.plus (term_unsigned (term_var "paddr")) (term_val ty.int (Z.of_nat bytes)) < (term_val ty.int (Z.of_N (bv.exp2 xlenbits))) (* ∗ *) *)
+        (*    (* asn_inv_mmio bytes ∗ *) *)
+        (*    (* asn_mmio_checked_write bytes (term_var "paddr") (term_var "data") *)) *)
+          (∃ "mem_val", term_var "paddr" ↦ₘ[ bytes ] term_var "mem_val" ∗
            (term_val ty.int (Z.of_N minAddr) <= term_unsigned (term_var "paddr"))%asn ∗
            (term_binop bop.plus (term_unsigned (term_var "paddr")) (term_val ty.int (Z.of_nat bytes))) <= term_val ty.int (Z.of_N maxAddr)) ∗
         asn_cur_privilege (term_val ty_privilege Machine) (* ∗ *)
         (* asn_pmp_entries (term_var "entries") ∗ *)
-        (* asn_pmp_access (term_var "paddr") (term_get_slice_int (term_val ty.int (Z.of_nat bytes))) (term_var "entries") (term_val ty_privilege Machine) (term_val ty_access_type Write) *);
+        (* asn_pmp_access (term_var "paddr") (term_get_slice_int (term_val ty.int (Z.of_nat bytes))) (term_var "entries") (term_val ty_privilege Machine) (term_val ty_access_type Write) *) ∗
+        asn.chunk (chunk_user inv_leakage [env]) ∗
+    asn.formula (formula_secLeak (term_var "paddr"));
       sep_contract_result          := "result_mem_write";
       sep_contract_postcondition   :=
         term_var "result_mem_write" = term_union (memory_op_result 1) KMemValue (term_val ty_byte [bv 1]) ∗
-        asn.match_bool (term_var "inv") ⊤ (term_var "paddr" ↦ₘ[ bytes ] term_var "data") ∗
+        (* asn.match_bool (term_var "inv") ⊤ *) (term_var "paddr" ↦ₘ[ bytes ] term_var "data") ∗
         asn_cur_privilege (term_val ty_privilege Machine) (* ∗ *)
         (* asn_pmp_entries (term_var "entries") *);
     |}.
@@ -476,24 +495,26 @@ Module RiscvPmpBlockVerifSpec <: Specification RiscvPmpBase RiscvPmpSignature Ri
   Qed.
 
   Definition sep_contract_read_ram {bytes} : SepContractFunX (read_ram bytes) :=
-    {| sep_contract_logic_variables := ["inv" :: ty.bool; "paddr" :: ty_xlenbits; "w" :: ty_bytes bytes];
+    {| sep_contract_logic_variables := ["inv" :: ty.bool; "paddr" :: ty_xlenbits; "ram_val" :: ty_bytes bytes];
        sep_contract_localstore      := [term_var "paddr"];
-       sep_contract_precondition    := asn.match_bool (term_var "inv")  (term_var "paddr" ↦ᵣ[ bytes ] term_var "w") (term_var "paddr" ↦ₘ[ bytes ] term_var "w");
+       sep_contract_precondition    :=
+        asn.match_bool (term_var "inv")  (term_var "paddr" ↦ᵣ[ bytes ] term_var "ram_val") (term_var "paddr" ↦ₘ[ bytes ] term_var "ram_val");
        sep_contract_result          := "result_read_ram";
-       sep_contract_postcondition   := asn.match_bool (term_var "inv")
-                                         (term_var "paddr" ↦ᵣ[ bytes ] term_var "w") (term_var "paddr" ↦ₘ[ bytes ] term_var "w") ∗
-                                            term_var "result_read_ram" = term_var "w";
+       sep_contract_postcondition   :=
+        asn.match_bool (term_var "inv")
+        (term_var "paddr" ↦ᵣ[ bytes ] term_var "ram_val") (term_var "paddr" ↦ₘ[ bytes ] term_var "ram_val") ∗
+        asn.formula (formula_propeq (term_var "result_read_ram") (term_var "ram_val"));
     |}.
 
   Definition sep_contract_write_ram {bytes} : SepContractFunX (write_ram bytes) :=
     {| sep_contract_logic_variables := ["paddr" :: ty_word; "data" :: ty_bytes bytes];
        sep_contract_localstore      := [term_var "paddr"; term_var "data"];
-       sep_contract_precondition    := ∃ "w", (asn.chunk (chunk_user (ptstomem bytes) [term_var "paddr"; term_var "w"]));
+       sep_contract_precondition    := ∃ "ram_val", (asn.chunk (chunk_user (ptstomem bytes) [term_var "paddr"; term_var "ram_val"]));
        sep_contract_result          := "result_write_ram";
        sep_contract_postcondition   :=  term_var "paddr" ↦ₘ[ bytes ] term_var "data";
     |}.
 
-  (* Note; we define the contract like this, because it matches the PRE of `checked_mem_read` quite well*)
+  (* Note; we define the contract like tvhis, because it matches the PRE of `checked_mem_read` quite well*)
   (* Definition sep_contract_within_mmio `(H : restrict_bytes bytes) : SepContractFunX (within_mmio H) := *)
   (*   {| sep_contract_logic_variables := ["inv" :: ty.bool; "paddr" :: ty_xlenbits]; *)
   (*       sep_contract_localstore      := [term_var "paddr"]; *)
@@ -528,6 +549,15 @@ Module RiscvPmpBlockVerifSpec <: Specification RiscvPmpBase RiscvPmpSignature Ri
        sep_contract_postcondition   := term_var "result_decode" = term_var "instr";
     |}.
 
+  Definition sep_contract_leak    : SepContractFunX leak :=
+    {| sep_contract_logic_variables := ["leak" :: ty_leak_event];
+      sep_contract_localstore      := [term_var "leak"];
+      sep_contract_precondition    := asn.chunk (chunk_user inv_leakage [env]) ∗
+    asn.formula (formula_secLeak (term_var "leak"));
+      sep_contract_result          := "result";
+      sep_contract_postcondition   := ⊤;
+    |}.
+
   Definition CEnvEx : SepContractEnvEx :=
     fun Δ τ f =>
       match f with
@@ -537,6 +567,7 @@ Module RiscvPmpBlockVerifSpec <: Specification RiscvPmpBase RiscvPmpSignature Ri
       (* | mmio_read bytes => sep_contract_mmio_read bytes *)
       (* | mmio_write res  => @sep_contract_mmio_write _ res *)
       | decode          => sep_contract_decode
+      | leak            => sep_contract_leak
       end.
 
   Lemma linted_cenvex :
@@ -564,15 +595,18 @@ Module RiscvPmpBlockVerifSpec <: Specification RiscvPmpBase RiscvPmpSignature Ri
     {| lemma_logic_variables := ["paddr" :: ty_word; "i" :: ty_ast];
        lemma_patterns        := [term_var "paddr"];
        lemma_precondition    := asn.chunk (chunk_user ptstoinstr [term_var "paddr"; term_var "i"]);
-      lemma_postcondition   := ∃ "w", (asn.chunk (chunk_user (ptstomem bytes_per_word) [term_var "paddr"; term_var "w"]) ∗
-                                      asn.chunk (chunk_user encodes_instr [term_var "w"; term_var "i"]))
+      lemma_postcondition   := ∃ "op", (asn.chunk (chunk_user (ptstomem bytes_per_word) [term_var "paddr"; term_var "op"]) ∗
+                                          asn.chunk (chunk_user encodes_instr [term_var "op"; term_var "i"]) ∗
+                                          asn.formula (formula_secLeak (term_var "op"))
+                                       )
     |}.
 
   Definition lemma_close_ptsto_instr : SepLemma close_ptsto_instr :=
-    {| lemma_logic_variables := ["paddr" :: ty_word; "w" :: ty_word; "i" :: ty_ast];
-       lemma_patterns        := [term_var "paddr"; term_var "w"];
-       lemma_precondition    := asn.chunk (chunk_user (ptstomem bytes_per_word) [term_var "paddr"; term_var "w"]) ∗
-                                  asn.chunk (chunk_user encodes_instr [term_var "w"; term_var "i"]);
+    {| lemma_logic_variables := ["paddr" :: ty_word; "cl" :: ty_word; "i" :: ty_ast];
+       lemma_patterns        := [term_var "paddr"; term_var "cl"];
+       lemma_precondition    := asn.chunk (chunk_user (ptstomem bytes_per_word) [term_var "paddr"; term_var "cl"]) ∗
+                                  asn.chunk (chunk_user encodes_instr [term_var "cl"; term_var "i"]) ∗
+                                  asn.formula (formula_secLeak (term_var "cl"));
        lemma_postcondition   := asn.chunk (chunk_user ptstoinstr [term_var "paddr"; term_var "i"]);
     |}.
 
@@ -665,16 +699,16 @@ Module RiscvPmpSpecVerif.
     | None => False
     end.
 
-
-  Definition test := (postprocess
-                       (SPureSpec.replay
-                          (postprocess (RiscvPmpBlockVerifExecutor.vcgen RiscvPmpBlockVerifExecutor.default_config 1 sep_contract_rX' fun_rX' wnil)))).
-
-  Import SymProp.notations.
-  Eval vm_compute in test.
+  Ltac symbolic_simpl :=
+    apply validcontract_with_erasure_sound;
+    vm_compute;
+    constructor;
+    cbn.
 
   Lemma valid_execute_rX : ValidContract rX.
-  Proof. vm_compute. Qed.
+  Proof.
+    now vm_compute.
+  Qed.
 
   Lemma valid_execute_wX : ValidContract wX.
   Proof. now vm_compute. Qed.
@@ -683,6 +717,7 @@ Module RiscvPmpSpecVerif.
   (* Set Printing Depth 200. *)
   (* Eval vm_compute in (postprocess (RiscvPmpBlockVerifExecutor.SHeapSpecM.vcgen RiscvPmpBlockVerifExecutor.default_config 1 *)
   (*            sep_contract_fetch_instr (FunDef fetch))). *)
+
   Lemma valid_execute_fetch : ValidContract fetch.
   Proof. now vm_compute. Qed.
 
@@ -692,13 +727,14 @@ Module RiscvPmpSpecVerif.
   Lemma valid_execute_tick_pc : ValidContract tick_pc.
   Proof. now vm_compute. Qed.
 
-  Ltac symbolic_simpl :=
-    apply validcontract_with_erasure_sound;
-    vm_compute;
-    constructor;
-    cbn.
 
   Import RiscvPmpBlockVerifExecutor.
+
+  (* Definition test := (postprocess *)
+  (*                       (SPureSpec.replay *)
+  (*                          (postprocess (RiscvPmpBlockVerifExecutor.vcgen RiscvPmpBlockVerifExecutor.default_config 1 sep_contract_read fun_checked_read wnil)))). *)
+  Import SymProp.notations.
+  (* Eval vm_compute in test. *)
 
   Lemma valid_checked_mem_read {bytes} {H : restrict_bytes bytes} : ValidContract (@checked_mem_read bytes H).
   Proof. destruct H; now vm_compute. Qed.
@@ -706,51 +742,51 @@ Module RiscvPmpSpecVerif.
   Lemma valid_checked_mem_write {bytes} {H : restrict_bytes bytes} : ValidContract (@checked_mem_write bytes H).
   Proof. destruct H; now vm_compute. Qed.
 
-  Lemma valid_pmp_mem_read {bytes} {H : restrict_bytes bytes} : ValidContract (@pmp_mem_read bytes H).
-  Proof. destruct H; now vm_compute. Qed.
+  (* Lemma valid_pmp_mem_read {bytes} {H : restrict_bytes bytes} : ValidContract (@pmp_mem_read bytes H). *)
+  (* Proof. destruct H; now vm_compute. Qed. *)
 
-  Lemma valid_pmp_mem_write {bytes} {H : restrict_bytes bytes} : ValidContract (@pmp_mem_write bytes H).
-  Proof. destruct H; now vm_compute. Qed.
+  (* Lemma valid_pmp_mem_write {bytes} {H : restrict_bytes bytes} : ValidContract (@pmp_mem_write bytes H). *)
+  (* Proof. destruct H; now vm_compute. Qed. *)
 
   Import Bitvector.bv.notations.
 
-  Lemma valid_pmpMatchAddr : ValidContractDebug pmpMatchAddr.
-  Proof.
-    symbolic_simpl.
-    intros; split; intros; bv_comp; auto.
-    destruct (v + v0 <=ᵘ? v1)%bv eqn:?; bv_comp; auto.
-  Qed.
+  (* Lemma valid_pmpMatchAddr : ValidContractDebug pmpMatchAddr. *)
+  (* Proof. *)
+  (*   symbolic_simpl. *)
+  (*   intros; split; intros; bv_comp; auto. *)
+  (*   destruct (v + v0 <=ᵘ? v1)%bv eqn:?; bv_comp; auto. *)
+  (* Qed. *)
 
-  Lemma valid_pmpCheck {bytes : nat} {H : restrict_bytes bytes} : ValidContractWithFuelDebug 4 (@pmpCheck bytes H).
-  Proof.
-    destruct H; apply verification_condition_with_erasure_sound; vm_compute;
-      constructor; cbn;
-      repeat (intros; split; intros);
-      repeat match goal with
-        | H: (?b1 || ?b2)%bool = true |- _ =>
-            apply Bool.orb_true_iff in H
-        | H: ?P /\ ?Q |- _ =>
-            destruct H
-        | H: ?P \/ ?Q |- _ =>
-            destruct H as [H|H]
-        | H: negb ?b = true |- _ =>
-            apply Bool.negb_true_iff in H;
-            subst
-        | H1: ?a <=ᵘ ?b, H2: ?b <ᵘ ?a |- False =>
-            unfold bv.ult, bv.ule in *; apply N.le_ngt in H1; apply (H1 H2)
-        end;
-      subst;
-      unfold Pmp_check_perms, decide_pmp_check_perms, pmp_check_RWX in *;
-      simpl in *;
-      try discriminate;
-      try Lia.lia.
-  Qed.
+  (* Lemma valid_pmpCheck {bytes : nat} {H : restrict_bytes bytes} : ValidContractWithFuelDebug 4 (@pmpCheck bytes H). *)
+  (* Proof. *)
+  (*   destruct H; apply verification_condition_with_erasure_sound; vm_compute; *)
+  (*     constructor; cbn; *)
+  (*     repeat (intros; split; intros); *)
+  (*     repeat match goal with *)
+  (*       | H: (?b1 || ?b2)%bool = true |- _ => *)
+  (*           apply Bool.orb_true_iff in H *)
+  (*       | H: ?P /\ ?Q |- _ => *)
+  (*           destruct H *)
+  (*       | H: ?P \/ ?Q |- _ => *)
+  (*           destruct H as [H|H] *)
+  (*       | H: negb ?b = true |- _ => *)
+  (*           apply Bool.negb_true_iff in H; *)
+  (*           subst *)
+  (*       | H1: ?a <=ᵘ ?b, H2: ?b <ᵘ ?a |- False => *)
+  (*           unfold bv.ult, bv.ule in *; apply N.le_ngt in H1; apply (H1 H2) *)
+  (*       end; *)
+  (*     subst; *)
+  (*     unfold Pmp_check_perms, decide_pmp_check_perms, pmp_check_RWX in *; *)
+  (*     simpl in *; *)
+  (*     try discriminate; *)
+  (*     try Lia.lia. *)
+  (* Qed. *)
 
   Lemma valid_mem_read {bytes} {H : restrict_bytes bytes} : ValidContract (@mem_read bytes H).
-  Proof. now destruct H. Qed.
+  Proof. destruct H; now vm_compute. Qed.
 
   Lemma valid_mem_write_value {bytes} {H : restrict_bytes bytes} : ValidContract (@mem_write_value bytes H).
-  Proof. now destruct H. Qed.
+  Proof. destruct H; now vm_compute. Qed.
 
   Lemma valid_contract_within_phys_mem : ValidContractDebug within_phys_mem.
   Proof. symbolic_simpl. intros. Lia.lia. Qed.
@@ -803,10 +839,10 @@ Module RiscvPmpSpecVerif.
     - refine (valid_contract _ H valid_mem_read).
     - refine (valid_contract _ H valid_checked_mem_read).
     - refine (valid_contract _ H valid_checked_mem_write).
-    - refine (valid_contract _ H valid_pmp_mem_read).
-    - refine (valid_contract _ H valid_pmp_mem_write).
-    - refine (valid_contract_with_fuel_debug _ _ H valid_pmpCheck).
-    - refine (valid_contract_debug _ H valid_pmpMatchAddr).
+    (* - refine (valid_contract _ H valid_pmp_mem_read). *)
+    (* - refine (valid_contract _ H valid_pmp_mem_write). *)
+    (* - refine (valid_contract_with_fuel_debug _ _ H valid_pmpCheck). *)
+    (* - refine (valid_contract_debug _ H valid_pmpMatchAddr). *)
     - refine (valid_contract _ H valid_mem_write_value).
     - refine (valid_contract _ H valid_execute_fetch).
     - refine (valid_contract_debug _ H valid_contract_execute_EBREAK).
@@ -816,18 +852,18 @@ End RiscvPmpSpecVerif.
 Module RiscvPmpIrisInstanceWithContracts.
   Include ProgramLogicOn RiscvPmpBase RiscvPmpSignature RiscvPmpProgram
     RiscvPmpBlockVerifSpec.
-  Include IrisInstanceWithContracts RiscvPmpBase RiscvPmpSignature
-    RiscvPmpProgram RiscvPmpSemantics RiscvPmpBlockVerifSpec RiscvPmpIrisBase
-    RiscvPmpIrisAdeqParameters
-    RiscvPmpIrisInstance.
+  Include IrisInstanceWithContracts2 RiscvPmpBase RiscvPmpSignature
+    RiscvPmpProgram RiscvPmpSemantics RiscvPmpBlockVerifSpec RiscvPmpIrisBase2
+    (* RiscvPmpIrisAdeqParameters *) RiscvPmpIrisAdeqParams2
+    RiscvPmpIrisInstance2.
   Include MicroSail.ShallowSoundness.Soundness RiscvPmpBase RiscvPmpSignature
     RiscvPmpProgram RiscvPmpBlockVerifSpec RiscvPmpBlockVerifShalExecutor.
   Include MicroSail.RefineExecutor.RefineExecOn RiscvPmpBase RiscvPmpSignature
     RiscvPmpProgram RiscvPmpBlockVerifSpec RiscvPmpBlockVerifShalExecutor
     RiscvPmpBlockVerifExecutor.
 
-  Import RiscvPmpIrisBase.
-  Import RiscvPmpIrisInstance.
+  Import RiscvPmpIrisBase2.
+  Import RiscvPmpIrisInstance2.
   Import RiscvPmp.Model.
 
   Import iris.bi.interface.
@@ -839,123 +875,206 @@ Module RiscvPmpIrisInstanceWithContracts.
   Import iris.proofmode.string_ident.
   Import iris.proofmode.tactics.
 
-  Lemma read_ram_sound `{sailGS Σ} {bytes} :
-    TValidContractForeign RiscvPmpBlockVerifSpec.sep_contract_read_ram (read_ram bytes).
+  Lemma read_ram_sound `{sailGS2 Σ} {bytes} :
+    ValidContractForeign RiscvPmpBlockVerifSpec.sep_contract_read_ram (read_ram bytes).
   Proof.
       intros Γ es δ ι Heq. cbn. destruct_syminstance ι.
-      iIntros "H". cbn in *. iApply semTWP_foreign.
-      iIntros (? ?) "(Hregs & % & Hmem & %Hmap & Htr)".
+      iIntros "H". cbn in *. iApply semWP2_foreign. unfold mem_inv2.
+      iIntros (? ? ? ?) "((Hregs1 & Hregs2) & ((%memmapL & HmemL & %HmapL & HtrL & HltrL) & (%memmapR & HmemR & %HmapR & HtrR & HltrR)))".
       iMod (fupd_mask_subseteq empty) as "Hclose"; auto. iModIntro.
-      iIntros (res ? ? Hf). rewrite Heq in Hf. cbn in Hf. inversion Hf; subst.
+      iIntros (resL ? ? resR ? ? Hf).
+      rewrite evalValsProjLeftIsProjLeftEvals in Hf. rewrite evalValsProjRightIsProjRightEvals in Hf.
+      rewrite Heq in Hf. cbn in Hf. inversion Hf; subst.
+      inversion H0; inversion H1; subst. clear H0 H1 Hf. do 3 iModIntro.
       iMod "Hclose" as "_". destruct inv.
-      - (* readonly case *)
+      { cbn. destruct v.
+        - (* readonly case *)
         iDestruct "H" as "#H".
-        iInv "H" as "Hptsto" "Hclose_ptsto".
-        iDestruct (bi.later_mono _ _ (RiscvPmpModel2.fun_read_ram_works Hmap) with "[$Hptsto $Hmem]") as "#>%eq_fun_read_ram".
-        iMod ("Hclose_ptsto" with "Hptsto") as "_". iModIntro.
-        iFrame "Hregs Hmem Htr". iSplitR; first auto.
-        iApply semTWP_val. iModIntro.
-        now iFrame "H".
+         iInv "H" as "Hptsto" "Hclose_ptsto".
+        iDestruct "Hptsto" as "(HptstoL & HptstoR)".
+        iDestruct (bi.later_mono _ _ (RiscvPmpModel2.fun_read_ram_works (sg := sailGS2_sailGS_left) HmapL) with "[$HptstoL $HmemL]") as "#>%eq_fun_read_ramL".
+        iDestruct (bi.later_mono _ _ (RiscvPmpModel2.fun_read_ram_works (sg := sailGS2_sailGS_right) HmapR) with "[$HptstoR $HmemR]") as "#>%eq_fun_read_ramR".
+        iMod ("Hclose_ptsto" with "[$HptstoL $HptstoR]") as "_".
+        iFrame "Hregs1 Hregs2 HmemL HmemR HtrL HltrL HtrR HltrR".
+        iSplitR; first auto.
+        iApply semWP2_val. do 2 iModIntro.
+        iExists δ. iSplitR; first auto.
+        destruct ram_val.
+        + iExists (SyncVal (fun_read_ram μ1 bytes (ty.projLeft paddr))). iSplitR; first by rewrite eq_fun_read_ramR.
+          iFrame "H".
+          iSplitR; try auto.
+          iSplitR; first auto.
+          by rewrite eq_fun_read_ramL.
+          auto. (* TODO: How to dispatch emp goal, also several admits for this below *)
+        + iExists (NonSyncVal (fun_read_ram μ1 bytes (ty.projLeft paddr)) (fun_read_ram μ2 bytes (ty.projRight paddr))). iSplitR; first by rewrite eq_fun_read_ramR.
+          iFrame "H".
+          iSplitR; try auto.
+          iSplitR; first auto.
+          by rewrite eq_fun_read_ramL eq_fun_read_ramR.
+          auto.
       - (* old case *)
         iModIntro.
-        iPoseProof (RiscvPmpModel2.fun_read_ram_works Hmap with "[$H $Hmem]") as "%eq_fun_read_ram".
-        iPoseProof (RiscvPmpModel2.mem_inv_not_modified $! Hmap with "Hmem Htr") as "Hmem".
-        iFrame "Hregs Hmem". iApply semTWP_val. now iFrame "H".
+        iDestruct "H" as "(HL & HR)".
+        iPoseProof (RiscvPmpModel2.fun_read_ram_works (sg := sailGS2_sailGS_left) HmapL with "[$HL $HmemL]") as "%eq_fun_read_ramL".
+        iPoseProof (RiscvPmpModel2.fun_read_ram_works (sg := sailGS2_sailGS_right) HmapR with "[$HR $HmemR]") as "%eq_fun_read_ramR".
+        iPoseProof (RiscvPmpModel2.mem_inv_not_modified (sg := sailGS2_sailGS_left) $! HmapL with "HmemL HtrL HltrL") as "HmemL".
+        iPoseProof (RiscvPmpModel2.mem_inv_not_modified (sg := sailGS2_sailGS_right) $! HmapR with "HmemR HtrR HltrR") as "HmemR".
+        iFrame "Hregs1 Hregs2 HmemL HmemR". iApply semWP2_val.
+        iFrame "HL". iFrame "HR".
+        iExists δ. iModIntro. iSplitR; first auto.
+        destruct ram_val.
+        + iExists (SyncVal (fun_read_ram μ1 bytes (ty.projLeft paddr))).
+          iSplitR; first by rewrite eq_fun_read_ramR.
+          iSplitR; try auto.
+          iSplitR; first by rewrite eq_fun_read_ramL.
+          auto.
+        + iExists (NonSyncVal (fun_read_ram μ1 bytes (ty.projLeft paddr)) (fun_read_ram μ2 bytes (ty.projRight paddr))). iSplitR; first by rewrite eq_fun_read_ramR.
+          iSplitR; try auto.
+          iSplitR; first auto.
+          by rewrite eq_fun_read_ramL eq_fun_read_ramR.
+          auto.
+      }
+      cbn. iDestruct "H" as "%". contradiction.
   Qed.
 
-  Lemma write_ram_sound `{sailGS Σ} {bytes} :
-    TValidContractForeign RiscvPmpBlockVerifSpec.sep_contract_write_ram (write_ram bytes).
+  Lemma write_ram_sound `{sailGS2 Σ} {bytes} :
+    ValidContractForeign RiscvPmpBlockVerifSpec.sep_contract_write_ram (write_ram bytes).
   Proof.
     intros Γ es δ ι Heq. destruct_syminstance ι. cbn in *.
-    iIntros "[%w H]". iApply semTWP_foreign.
-    iIntros (? ?) "(Hregs & % & Hmem & %Hmap & Htr)".
+    iIntros "[%w (HL & HR)]". iApply semWP2_foreign.
+    iIntros (? ? ? ?) "((Hregs1 & Hregs2) & ((%memmapL & HmemL & %HmapL & HtrL) & (%memmapR & HmemR & %HmapR & HtrR)))".
     iMod (fupd_mask_subseteq empty) as "Hclose"; auto. iModIntro.
-    iIntros (res ? ? Hf). rewrite Heq in Hf. cbn in Hf. inversion Hf; subst.
+    iIntros (res1 ? ? res2 ? ? Hf).
+    rewrite evalValsProjLeftIsProjLeftEvals in Hf. rewrite evalValsProjRightIsProjRightEvals in Hf.
+    rewrite Heq in Hf. cbn in Hf. inversion Hf; subst.
+    inversion H0; inversion H1; subst. clear H0 H1 Hf. do 3 iModIntro.
     iMod "Hclose" as "_".
-    iMod (RiscvPmpModel2.fun_write_ram_works with "[$H $Hmem $Htr]") as "[$ H]"; auto.
-    rewrite semTWP_val. now iFrame "Hregs H".
+    iMod (RiscvPmpModel2.fun_write_ram_works (sg := sailGS2_sailGS_left) with "[$HL $HmemL $HtrL]") as "[$ HL]"; auto.
+    iMod (RiscvPmpModel2.fun_write_ram_works (sg := sailGS2_sailGS_right) with "[$HR $HmemR $HtrR]") as "[$ HR]"; auto.
+    rewrite semWP2_val. iFrame "Hregs1 Hregs2".
+    iExists δ. iSplitR; first auto.
+    iExists (SyncVal true). iSplitR; first auto. by iFrame "HL HR".
  Qed.
 
   (* Important sanity condition on mmio predicates - NOTE: could be in typeclass, together with the condition that reads are either all accepted, or none of them are *)
   Lemma mmio_pred_cons {bytes : nat} t e: event_pred bytes e → mmio_pred bytes t → mmio_pred bytes (cons e t).
   Proof. now apply List.Forall_cons. Qed.
 
-  Lemma mmio_write_sound `{!sailGS Σ} `(H: restrict_bytes bytes) :
-    TValidContractForeign (@RiscvPmpBlockVerifSpec.sep_contract_mmio_write _ H) (mmio_write H).
-  Proof.
-    intros Γ es δ ι Heq. destruct_syminstance ι. cbn in *.
-    iIntros "([%Hmmio _] & #Hinv & [-> ->])". iApply semTWP_foreign.
-    iIntros (? ?) "[Hregs [% (Hmem & %Hmap & Htr)]]".
-    iInv "Hinv" as (t) " [>Htrf >%Hpred]" "Hclose".
-    iDestruct (trace.trace_full_frag_eq with "Htr Htrf") as "%Heqt". subst t.
-    iMod (trace.trace_update _ _ (cons _ _) with "[$Htr $Htrf]") as "[Htr Htrf]".
-    iMod ("Hclose" with "[Htrf]") as "_".
-    {(* Instantiate evars *)
-      iExists _; iFrame. iPureIntro.
-      apply mmio_pred_cons; [|eauto].
-      constructor. }
-    iMod (fupd_mask_subseteq empty) as "Hclose"; auto. iModIntro.
-    iIntros (res ? ? Hf). rewrite Heq in Hf. cbn in Hf. inversion Hf; subst.
-    iMod "Hclose" as "_". rewrite semTWP_val.
-    destruct bytes; first contradiction.
-    unfold mem_inv, fun_write_mmio; cbn.
-    now iFrame "Hregs Hmem Htr".
-  Qed.
+  (* Lemma mmio_write_sound `{!sailGS Σ} `(H: restrict_bytes bytes) : *)
+  (*   TValidContractForeign (@RiscvPmpBlockVerifSpec.sep_contract_mmio_write _ H) (mmio_write H). *)
+  (* Proof. *)
+  (*   intros Γ es δ ι Heq. destruct_syminstance ι. cbn in *. *)
+  (*   iIntros "([%Hmmio _] & #Hinv & [-> ->])". iApply semTWP_foreign. *)
+  (*   iIntros (? ?) "[Hregs [% (Hmem & %Hmap & Htr)]]". *)
+  (*   iInv "Hinv" as (t) " [>Htrf >%Hpred]" "Hclose". *)
+  (*   iDestruct (trace.trace_full_frag_eq with "Htr Htrf") as "%Heqt". subst t. *)
+  (*   iMod (trace.trace_update _ _ (cons _ _) with "[$Htr $Htrf]") as "[Htr Htrf]". *)
+  (*   iMod ("Hclose" with "[Htrf]") as "_". *)
+  (*   {(* Instantiate evars *) *)
+  (*     iExists _; iFrame. iPureIntro. *)
+  (*     apply mmio_pred_cons; [|eauto]. *)
+  (*     constructor. } *)
+  (*   iMod (fupd_mask_subseteq empty) as "Hclose"; auto. iModIntro. *)
+  (*   iIntros (res ? ? Hf). rewrite Heq in Hf. cbn in Hf. inversion Hf; subst. *)
+  (*   iMod "Hclose" as "_". rewrite semTWP_val. *)
+  (*   destruct bytes; first contradiction. *)
+  (*   unfold mem_inv, fun_write_mmio; cbn. *)
+  (*   now iFrame "Hregs Hmem Htr". *)
+  (* Qed. *)
 
-  Lemma decode_sound `{sailGS Σ} :
-    TValidContractForeign RiscvPmpBlockVerifSpec.sep_contract_decode RiscvPmpProgram.decode.
+  Lemma decode_sound `{sailGS2 Σ} :
+    ValidContractForeign RiscvPmpBlockVerifSpec.sep_contract_decode RiscvPmpProgram.decode.
   Proof.
     intros Γ es δ ι Heq. destruct_syminstance ι. cbn in *.
-    iIntros "%Hdecode". iApply semTWP_foreign.
-    iIntros (? ?) "[Hregs [% (Hmem & %Hmap & Htr)]]".
+    iIntros "%Hdecode". iApply semWP2_foreign.
+    iIntros (? ? ? ?) "((Hregs1 & Hregs2) & ((%memmapL & HmemL & %HmapL & HtrL & HltrL) & (%memmapR & HmemR & %HmapR & HtrR & HltrR)))".
     iMod (fupd_mask_subseteq empty) as "Hclose"; auto. iModIntro.
-    iIntros (? ? ? Hf). iMod "Hclose" as "_".
+    iIntros (res1 ? ? res2 ? ? Hf).
+    rewrite evalValsProjLeftIsProjLeftEvals in Hf. rewrite evalValsProjRightIsProjRightEvals in Hf.
     rewrite Heq in Hf. cbn in Hf. inversion Hf; subst.
+    inversion H0; inversion H1; subst. clear H0 H1 Hf. do 3 iModIntro.
+    iMod "Hclose" as "_".
+    iPoseProof (RiscvPmpModel2.mem_inv_not_modified (sg := sailGS2_sailGS_left) $! HmapL with "HmemL HtrL HltrL") as "HmemL".
+    iPoseProof (RiscvPmpModel2.mem_inv_not_modified (sg := sailGS2_sailGS_right) $! HmapR with "HmemR HtrR HltrR") as "HmemR".
+    iFrame "Hregs1 Hregs2 HmemL HmemR".
+    destruct code; destruct instr; cbn in *;
     destruct (pure_decode _); inversion Hdecode.
-    iPoseProof (RiscvPmpModel2.mem_inv_not_modified $! Hmap with "Hmem Htr") as "Hmem".
-    rewrite semTWP_val. now iFrame "Hregs Hmem".
+    + rewrite semWP2_val.
+      iExists δ. iSplitR; first auto. iExists (SyncVal v0). auto.
+    + destruct (pure_decode); inversion Hdecode.
+      rewrite semWP2_val.
+      iExists δ. iSplitR; first auto. iExists (NonSyncVal v1 v2). auto.
   Qed.
 
-  Lemma within_mmio_sound `{!sailGS Σ} `(H: restrict_bytes bytes):
-    TValidContractForeign (RiscvPmpBlockVerifSpec.sep_contract_within_mmio H) (RiscvPmpProgram.within_mmio H).
+  (* Lemma within_mmio_sound `{!sailGS Σ} `(H: restrict_bytes bytes): *)
+  (*   TValidContractForeign (RiscvPmpBlockVerifSpec.sep_contract_within_mmio H) (RiscvPmpProgram.within_mmio H). *)
+  (* Proof. *)
+  (*   intros Γ es δ ι Heq. destruct_syminstance ι. cbn in *. *)
+  (*   iIntros "Hpre". iApply semTWP_foreign. *)
+  (*   iIntros (? ?) "(Hregs & Hmem)". *)
+  (*   iMod (fupd_mask_subseteq empty) as "Hclose"; auto. iModIntro. *)
+  (*   iIntros (? ? ? Hf). rewrite Heq in Hf. cbn in Hf. inversion Hf; subst. *)
+  (*   rewrite semTWP_val. iMod "Hclose" as "_". iFrame "Hregs Hmem". *)
+  (*   repeat iModIntro. *)
+  (*   rewrite /fun_within_mmio bool_decide_and. *)
+  (*   destruct inv; cbn; iDestruct "Hpre" as "([%Hlft _] & [%Hrght _])". *)
+  (*   - iPureIntro; repeat split; auto. *)
+  (*     rewrite -bool_decide_and bool_decide_true //. *)
+  (*     split; [auto| solve_bv]. *)
+  (*   - iPureIntro; repeat split; auto. *)
+  (*     assert (bool_decide (withinMMIO paddr bytes) = false) as ->. *)
+  (*     { rewrite bool_decide_eq_false. *)
+  (*       destruct bytes; first easy. *)
+  (*       assert (paddr ∈ liveAddrs)%stdpp. *)
+  (*       { apply bv.in_seqBv. *)
+  (*         - change (bv.of_N minAddr) with (@bv.zero xlenbits); cbn. (* TODO: add simplifying `xlenbits` to solve_bv *) solve_bv. *)
+  (*         - rewrite N2Z.inj_add in Hrght. *)
+  (*           change minAddr with 0%N in *; cbn in *. *)
+  (*           assert (bv.unsigned paddr < Z.of_N lenAddr)%Z by Lia.lia. cbn. *)
+  (*           cbv [bv.ult]. now zify. (* `solve_bv` fails because knowledge of concrete `minAddr`, `lenAddr` needed *)} *)
+  (*       intros HFalse; cbn in HFalse. *)
+  (*       assert (paddr ∈ mmioAddrs)%stdpp by (destruct bytes; intuition). *)
+  (*       eapply mmio_ram_False; eauto. *)
+  (*     } *)
+  (*     auto. *)
+  (* Qed. *)
+
+    Lemma leak_sound `{sailGS2 Σ} :
+    ValidContractForeign RiscvPmpBlockVerifSpec.sep_contract_leak RiscvPmpProgram.leak.
   Proof.
     intros Γ es δ ι Heq. destruct_syminstance ι. cbn in *.
-    iIntros "Hpre". iApply semTWP_foreign.
-    iIntros (? ?) "(Hregs & Hmem)".
+    iIntros "(Hinv & %HsL & _)". iApply semWP2_foreign.
+    iIntros (? ? ? ?) "((Hregs1 & Hregs2) & ((%memmapL & HmemL & %HmapL & HtrL & HltrL) & (%memmapR & HmemR & %HmapR & HtrR & HltrR)))".
     iMod (fupd_mask_subseteq empty) as "Hclose"; auto. iModIntro.
-    iIntros (? ? ? Hf). rewrite Heq in Hf. cbn in Hf. inversion Hf; subst.
-    rewrite semTWP_val. iMod "Hclose" as "_". iFrame "Hregs Hmem".
-    repeat iModIntro.
-    rewrite /fun_within_mmio bool_decide_and.
-    destruct inv; cbn; iDestruct "Hpre" as "([%Hlft _] & [%Hrght _])".
-    - iPureIntro; repeat split; auto.
-      rewrite -bool_decide_and bool_decide_true //.
-      split; [auto| solve_bv].
-    - iPureIntro; repeat split; auto.
-      assert (bool_decide (withinMMIO paddr bytes) = false) as ->.
-      { rewrite bool_decide_eq_false.
-        destruct bytes; first easy.
-        assert (paddr ∈ liveAddrs)%stdpp.
-        { apply bv.in_seqBv.
-          - change (bv.of_N minAddr) with (@bv.zero xlenbits); cbn. (* TODO: add simplifying `xlenbits` to solve_bv *) solve_bv.
-          - rewrite N2Z.inj_add in Hrght.
-            change minAddr with 0%N in *; cbn in *.
-            assert (bv.unsigned paddr < Z.of_N lenAddr)%Z by Lia.lia. cbn.
-            cbv [bv.ult]. now zify. (* `solve_bv` fails because knowledge of concrete `minAddr`, `lenAddr` needed *)}
-        intros HFalse; cbn in HFalse.
-        assert (paddr ∈ mmioAddrs)%stdpp by (destruct bytes; intuition).
-        eapply mmio_ram_False; eauto.
-      }
-      auto.
+    iIntros (res1 ? ? res2 ? ? Hf).
+    rewrite evalValsProjLeftIsProjLeftEvals in Hf. rewrite evalValsProjRightIsProjRightEvals in Hf.
+    rewrite Heq in Hf. cbn in Hf. inversion Hf; subst.
+    inversion H0; inversion H1; subst. clear H0 H1 Hf. do 3 iModIntro.
+    iMod "Hclose" as "_".
+    iInv "Hinv" as (t) " [>HltrfL >HltrfR]" "Hclose".
+    iPoseProof (trace.trace_full_frag_eq with "HltrL HltrfL") as "%eqL".
+    iPoseProof (trace.trace_full_frag_eq with "HltrR HltrfR") as "%eqR".
+    cbn. subst t.
+    rewrite eqR.
+    iMod (trace.trace_update _ _ (cons _ _) with "[$HltrL $HltrfL]") as "[HltrL HltrfL]".
+    iMod (trace.trace_update _ _ (cons _ _) with "[$HltrR $HltrfR]") as "[HltrR HltrfR]".
+    iMod ("Hclose" with "[$HltrfL $HltrfR]") as "_".
+    iPoseProof (RiscvPmpModel2.mem_inv_not_modified (sg := sailGS2_sailGS_left) (fun_leak μ1 (ty.projLeft leak0)) $! HmapL with "HmemL HtrL HltrL") as "HmemL".
+    rewrite <- eqR.
+    iPoseProof (RiscvPmpModel2.mem_inv_not_modified (sg := sailGS2_sailGS_right) (fun_leak μ2 (ty.projLeft leak0)) $! HmapR with "HmemR HtrR HltrR") as "HmemR".
+    apply secLeakOtherDef in HsL. rewrite HsL. cbn.
+    iFrame "Hregs1 Hregs2 HmemL HmemR".
+    rewrite semWP2_val.
+    iExists δ. iSplitR; first auto. iExists (SyncVal tt). auto.
   Qed.
 
-  Lemma TforeignSemBlockVerif `{sailGS Σ} : TForeignSem.
+  Lemma foreignSemBlockVerif `{sailGS2 Σ} : ForeignSem.
     intros Δ τ f; destruct f;
-        eauto using read_ram_sound, write_ram_sound, RiscvPmpModel2.mmio_read_sound, mmio_write_sound, within_mmio_sound, decode_sound.
+        eauto using read_ram_sound, write_ram_sound, (* RiscvPmpModel2.mmio_read_sound, mmio_write_sound, within_mmio_sound, *) decode_sound, leak_sound.
   Qed.
 
-  Lemma foreignSemBlockVerif `{sailGS Σ} : ForeignSem.
-  Proof. apply (TForeignSem_ForeignSem TforeignSemBlockVerif). Qed.
+  (* Lemma foreignSemBlockVerif `{sailGS Σ} : ForeignSem. *)
+  (* Proof. apply (TForeignSem_ForeignSem TforeignSemBlockVerif). Qed. *)
 
   Ltac destruct_syminstance ι :=
     repeat
@@ -970,59 +1089,59 @@ Module RiscvPmpIrisInstanceWithContracts.
       | _ => idtac
       end.
 
-  Lemma open_ptsto_instr_sound `{sailGS Σ} :
+  Lemma open_ptsto_instr_sound `{sailGS2 Σ} :
     ValidLemma RiscvPmpBlockVerifSpec.lemma_open_ptsto_instr.
   Proof.
     intros ι; destruct_syminstance ι; cbn.
-    iIntros "[%w (Hptsto & Henc )]".
-    iExists w.
+    iIntros "[%op (Hptsto & Henc & HsL )]".
+    iExists op.
     now iFrame.
   Qed.
 
-  Lemma close_ptsto_instr_sound `{sailGS Σ} :
+  Lemma close_ptsto_instr_sound `{sailGS2 Σ} :
     ValidLemma RiscvPmpBlockVerifSpec.lemma_close_ptsto_instr.
   Proof.
     intros ι; destruct_syminstance ι; cbn.
-    iIntros "(Hptsto & Henc )".
-    iExists w.
+    iIntros "(Hptsto & Henc & HsL & _)".
+    iExists cl.
     now iFrame.
   Qed.
 
-  Lemma close_mmio_write_sound `{sailGS Σ} (imm : bv 12) (width : WordWidth):
-    ValidLemma (RiscvPmpBlockVerifSpec.lemma_close_mmio_write imm width).
-  Proof.
-    intros ι; destruct_syminstance ι; cbn.
-    iIntros "([<- _] & [-> _])".
-    unfold interp_mmio_checked_write.
-    iPureIntro.
-    split; auto.
-    destruct width; now compute.
-  Qed.
+  (* Lemma close_mmio_write_sound `{sailGS Σ} (imm : bv 12) (width : WordWidth): *)
+  (*   ValidLemma (RiscvPmpBlockVerifSpec.lemma_close_mmio_write imm width). *)
+  (* Proof. *)
+  (*   intros ι; destruct_syminstance ι; cbn. *)
+  (*   iIntros "([<- _] & [-> _])". *)
+  (*   unfold interp_mmio_checked_write. *)
+  (*   iPureIntro. *)
+  (*   split; auto. *)
+  (*   destruct width; now compute. *)
+  (* Qed. *)
 
-  Lemma lemSemBlockVerif `{sailGS Σ} : LemmaSem.
+  Lemma lemSemBlockVerif `{sailGS2 Σ} : LemmaSem.
   Proof.
     intros Δ []; intros ι; destruct_syminstance ι; try now iIntros "_".
-    - apply Model.RiscvPmpModel2.open_pmp_entries_sound.
-    - apply Model.RiscvPmpModel2.close_pmp_entries_sound.
+    (* - apply Model.RiscvPmpModel2.open_pmp_entries_sound. *)
+    (* - apply Model.RiscvPmpModel2.close_pmp_entries_sound. *)
     - apply open_ptsto_instr_sound.
     - apply close_ptsto_instr_sound.
-    - apply close_mmio_write_sound.
+    (* - apply close_mmio_write_sound. *)
   Qed.
 
   Import RiscvPmpBlockVerifSpec.
   Import RiscvPmpBlockVerifExecutor.Symbolic.
 
-  Lemma TcontractsSound `{sailGS Σ} : ⊢ TValidContractEnvSem RiscvPmpBlockVerifSpec.CEnv.
-  Proof.
-    apply (tsound TforeignSemBlockVerif lemSemBlockVerif).
-    intros Γ τ f c Heq.
-    pose proof (RiscvPmpSpecVerif.ValidContracts f Heq) as [fuel Hvc].
-    eapply shallow_vcgen_fuel_soundness, symbolic_vcgen_fuel_soundness.
-    eauto.
-  Qed.
+  (* Lemma TcontractsSound `{sailGS Σ} : ⊢ TValidContractEnvSem RiscvPmpBlockVerifSpec.CEnv. *)
+  (* Proof. *)
+  (*   apply (tsound TforeignSemBlockVerif lemSemBlockVerif). *)
+  (*   intros Γ τ f c Heq. *)
+  (*   pose proof (RiscvPmpSpecVerif.ValidContracts f Heq) as [fuel Hvc]. *)
+  (*   eapply shallow_vcgen_fuel_soundness, symbolic_vcgen_fuel_soundness. *)
+  (*   eauto. *)
+  (* Qed. *)
 
   (* TODO: prove this lemma as: apply (TValidContractEnvSem_ValidContractEnvSem TcontractsSound). *)
-  Lemma contractsSound `{sailGS Σ} : ⊢ ValidContractEnvSem RiscvPmpBlockVerifSpec.CEnv.
+  Lemma contractsSound `{sailGS2 Σ} : ⊢ ValidContractEnvSem RiscvPmpBlockVerifSpec.CEnv.
   Proof.
     apply (sound foreignSemBlockVerif lemSemBlockVerif).
     intros Γ τ f c Heq.
